partial_abort/formalization/partialImpliesFull.v
@@ -23,33 +23,19 @@ Ltac solveByInv :=
       |H:_ |- _ => solve[inv H]
   end. 
 
-Theorem validateDeterministic : forall S L H S' S'' H' H'' L' L'' res res', 
-                                  validate S L H S' H' L' res ->
-                                  validate S L H S'' H'' L'' res' ->
-                                  L' = L'' /\ res = res'. 
+Theorem validateSameAns : forall L S H S' S'' e L' H', 
+                                  validate S L H S' (abort L' e) ->
+                                  validate S L H S'' (commit H') ->
+                                  False. 
 Proof.
-  intros. genDeps {{ S''; H''; L''; res' }}. induction H0; intros. 
-  {inv H1. auto. }
-  {inv H3; auto. apply IHvalidate in H13. invertHyp. inv H3. 
-   eapply lookupDeterministic in H15; eauto. invertHyp. omega. }
-  {inv H1. 
-   {apply IHvalidate in H13. invertHyp. inv H2. }
-   {apply IHvalidate in H11; eauto. }
-   {apply IHvalidate in H5; eauto. invertHyp. solveByInv. }
-   {apply IHvalidate in H11; eauto. invertHyp. solveByInv. }
-  }
-  {inv H3. 
-   {eapply lookupDeterministic in H1; eauto. invertHyp. omega. }
-   {apply IHvalidate in H13; eauto. invertHyp. solveByInv. }
-   {eapply lookupDeterministic in H1; eauto. }
-  }
-  {inv H1. eapply IHvalidate in H11; eauto. invertHyp. solveByInv. 
-   eapply IHvalidate in H12; eauto. }
+  induction L; intros. 
+  {inv H0. }
+  {inv H0; inv H1; eauto. eapply lookupDeterministic in H11; eauto. invertHyp. omega. }
 Qed. 
 
 Theorem transImpliesfMulti : forall C H C' S' S e e0 e' L L',
                   trans_multistep H (Some(S,e0),L,e) (Some(S,e0),L',e') -> 
-                  (exists H', validate S L H S' H' L commit) ->
+                  (exists H', validate S L H S' (commit H')) ->
                   C > S -> C' > C ->
                   f_multistep C' H (Single (Some(C,e0),L,e)) 
                               C' H (Single (Some(C,e0),L',e')). 
@@ -72,6 +58,17 @@ Proof.
   }
 Qed. 
 
+Theorem abortSameAns : forall S L H S' L' e' S'' L'' e'', 
+                         validate S L H S' (abort e' L') ->
+                         validate S L H S'' (abort e'' L'') ->
+                         e' = e'' /\ L' = L''. 
+Proof.
+  induction L; intros. 
+  {inv H0. }
+  {inv H0; inv H1; eauto. eapply validateSameAns in H10; eauto. inv H10. 
+   eapply validateSameAns in H10; eauto. inv H10. }
+Qed. 
+
 Theorem partialImpliesFull : forall C H T C' H' T', 
                                p_step C H T C' H' T' -> poolWF C H T ->
                                f_multistep C H T C' H' T'. 
@@ -84,11 +81,11 @@ Proof.
    eapply f_multi_R. eassumption. }
   {econstructor. eapply f_forkStep; eauto. constructor. }
   {inv H1. InTac. invertHyp. simpl in H1. inv H2. 
-   {eapply validateDeterministic in H0; eauto. invertHyp. solveByInv. }
-   {copy H0. eapply validateDeterministic in H0. Focus 2. eapply H7. invertHyp. 
-    inv H6. econstructor. eapply f_abortStep; eauto. 
+   {eapply validateSameAns in H0; eauto. inv H0. }
+   {copy H0. eapply abortSameAns in H7; eauto. invertHyp. 
+    econstructor. eapply f_abortStep; eauto. 
     apply validateValidate in H2. invertHyp. eapply transImpliesfMulti. eauto. 
-    econstructor. econstructor. auto. auto. }
+    econstructor. econstructor. eauto. auto. }
   }
   {econstructor. eapply f_allocStep; eauto. constructor. }
   {econstructor. eapply f_commitStep; eauto. constructor. }
